Initial version of the theory of separation logic.

theories/theories/utp_sep_logic.thy
@@ -4,12 +4,77 @@ begin
 
 default_sort STORE_SORT
 
+type_synonym ('a, 'm) PTR = "('a PADDR, 'm) PVAR"
+
 abbreviation "heap \<equiv> MkPlainP ''heap'' True TYPE('m STORE) TYPE('m :: STORE_SORT)"
 
-lift_definition AssignS :: "(ADDR, 'm) PVAR \<Rightarrow> 'm WF_EXPRESSION \<Rightarrow> 'm WF_PREDICATE" ("[_] := _" [0, 190] 190) is
-"\<lambda> x e. {b. \<langle>b\<rangle>\<^sub>* heap\<acute> = (\<langle>b\<rangle>\<^sub>* heap)(\<langle>b\<rangle>\<^sub>*x :=\<^sub>s \<lbrakk>e\<rbrakk>\<^sub>eb)}" .
+lift_definition AssignSR :: "('a, 'm) PTR \<Rightarrow> ('a, 'm) WF_PEXPRESSION \<Rightarrow> 'm WF_PREDICATE" ("[_] :=\<^sub>R _" [0, 190] 190) is
+"\<lambda> x e. {b. \<langle>b\<rangle>\<^sub>* heap\<acute> = (\<langle>b\<rangle>\<^sub>* heap)(\<langle>b\<rangle>\<^sub>*x :=\<^sub>& \<lbrakk>e\<rbrakk>\<^sub>*b)}" .
 
-term "[x] := v"
+lift_definition DeRefPE :: "('a, 'm) PTR \<Rightarrow> ('a, 'm) WF_PEXPRESSION"
+is "\<lambda> x b. \<langle>\<langle>b\<rangle>\<^sub>* heap\<rangle>\<^sub>& (\<langle>b\<rangle>\<^sub>*x)" .
+
+definition scomp_join :: "'m STORE \<Rightarrow> ('m STORE * 'm STORE) \<Rightarrow> bool" (infix "\<oast>" 50)
+where "scomp_join = (\<lambda> hp (h1, h2). sdom(h1) \<inter>\<^sub>f sdom(h2) = \<lbrace>\<rbrace> \<and> hp = h1 + h2)"
+
+lemma finter_commute: "x \<inter>\<^sub>f y = y \<inter>\<^sub>f x"
+  by auto
+
+lemma sdom_0 [simp]: "sdom(0) = \<lbrace>\<rbrace>"
+  by (metis fdom_fmempty sdom.rep_eq zero_STORE.rep_eq)
+
+lemma sran_0 [simp]: "sran(0) = \<lbrace>\<rbrace>"
+  by (auto simp add:sran.rep_eq zero_STORE.rep_eq fran.rep_eq zero_fmap.rep_eq)
+
+lemma scomp_join_id: "h \<oast> (h, 0)"
+  by (simp add:scomp_join_def)
+
+lemma scomp_join_sym: "h \<oast> (h1, h2) \<Longrightarrow> h \<oast> (h2, h1)"
+  apply (simp add:scomp_join_def, clarify)
+  apply (rule conjI)
+  apply (simp add: finter_commute)
+  apply (metis STORE_add_comm)
+done
+
+definition
+  CompJoinPE :: " ('m STORE, 'm::STORE_SORT) WF_PEXPRESSION 
+                \<Rightarrow> ('m STORE, 'm) WF_PEXPRESSION
+                \<Rightarrow> ('m STORE, 'm) WF_PEXPRESSION
+                \<Rightarrow> 'm WF_PREDICATE" where
+"CompJoinPE hp h1 h2 = (PExprP (Op2PE scomp_join hp (ProdPE h1 h2)))"
+
+declare CompJoinPE_def [evalp]
+
+syntax
+  "_upred_assignsr"  :: "('a, 'm) PTR \<Rightarrow> pexpr \<Rightarrow> upred" ("[_] := _" [100] 100)
+  "_upred_comp_join" :: "pexpr \<Rightarrow> pexpr \<Rightarrow> pexpr \<Rightarrow> upred" ("_ \<oast> '(_, _')" [59,0,0] 60)
+  "_pexpr_deref"     :: "('a, 'm) PTR \<Rightarrow> pexpr" ("[_]")
+
+translations
+  "_upred_assignsr x e"       == "CONST AssignSR x e"
+  "_upred_comp_join hp h1 h2" == "CONST CompJoinPE hp h1 h2"
+
+definition SepAndP :: "'a WF_PREDICATE \<Rightarrow> 'a WF_PREDICATE \<Rightarrow> 'a WF_PREDICATE" where
+"SepAndP p q = `\<exists>\<^sub>s h1. \<exists>\<^sub>s h2. ($heap \<oast> (\<guillemotleft>h1\<guillemotright>, \<guillemotleft>h2\<guillemotright>) \<and> p[\<guillemotleft>h1\<guillemotright>/heap] \<and> q[\<guillemotleft>h2\<guillemotright>/heap])`"
+
+declare SepAndP_def [eval, evalpp]
+
+syntax
+  "_upred_sep_and"   :: "upred \<Rightarrow> upred \<Rightarrow> upred" (infixr "*" 35)
+
+translations
+  "_upred_sep_and p q" == "CONST SepAndP p q"
+
+declare EvalP_ExistsShP [evalpp]
+declare EvalP_ForallShP [evalpp]
+
+lemma SepAndP_true: "`p * true` = `p`"
+  apply (simp add:SepAndP_def usubst)
+  apply (utp_poly_auto_tac)
+oops
+
+lemma SepAndP_comm: "`p * q` = `q * p`"
+  by (utp_poly_tac, metis scomp_join_sym)
 
 
 (*
